specs/.lake/build/ir/Fastvid.c
@@ -13,9 +13,11 @@
 #ifdef __cplusplus
 extern "C" {
 #endif
+LEAN_EXPORT lean_object* l_Fastvid_defaultTileWavefrontRounds;
 LEAN_EXPORT lean_object* l_Fastvid_PredictionMode_noConfusion___redArg___boxed(lean_object*, lean_object*);
 LEAN_EXPORT lean_object* l_Fastvid_riceDivisor___boxed(lean_object*);
 static lean_object* l_Fastvid_reprPredictionMode___closed__6____x40_Fastvid___hyg_406_;
+LEAN_EXPORT lean_object* l_Fastvid_riceLaneIndex(lean_object*, lean_object*);
 LEAN_EXPORT lean_object* l_Fastvid_ransTableSize(lean_object*);
 static lean_object* l_Fastvid_reprPredictionMode___closed__4____x40_Fastvid___hyg_406_;
 static lean_object* l_Fastvid_reprPredictionMode___closed__3____x40_Fastvid___hyg_406_;
@@ -32,23 +34,29 @@ LEAN_EXPORT lean_object* l_Fastvid_predictionModeCode___boxed(lean_object*);
 LEAN_EXPORT lean_object* l_Fastvid_PredictionMode_toCtorIdx(uint8_t);
 LEAN_EXPORT lean_object* l_Fastvid_riceDivisor(lean_object*);
 lean_object* lean_nat_shiftr(lean_object*, lean_object*);
+LEAN_EXPORT lean_object* l_Fastvid_parallelShardSymbols;
+LEAN_EXPORT lean_object* l_Fastvid_riceLaneIndex___boxed(lean_object*, lean_object*);
 LEAN_EXPORT lean_object* l___private_Fastvid_0__Fastvid_zigzag_match__1_splitter___boxed(lean_object*, lean_object*, lean_object*, lean_object*);
 static lean_object* l_Fastvid_reprPredictionMode___closed__1____x40_Fastvid___hyg_406_;
 LEAN_EXPORT lean_object* l___private_Fastvid_0__Fastvid_zigzag_match__1_splitter___redArg___closed__0;
 uint8_t lean_nat_dec_eq(lean_object*, lean_object*);
 LEAN_EXPORT lean_object* l_Fastvid_ransStateIndex(lean_object*, lean_object*);
+static lean_object* l_Fastvid_maximumParallelBlockBodyBytes___closed__0;
 lean_object* lean_nat_to_int(lean_object*);
+LEAN_EXPORT lean_object* l_Fastvid_predictorBandIndex(lean_object*);
 lean_object* lean_nat_div(lean_object*, lean_object*);
 static lean_object* l_Fastvid_reprPredictionMode___closed__2____x40_Fastvid___hyg_406_;
 LEAN_EXPORT lean_object* l_Fastvid_average2(lean_object*, lean_object*);
 LEAN_EXPORT lean_object* l_Fastvid_fixedWidthModulus___boxed(lean_object*);
 LEAN_EXPORT lean_object* l___private_Fastvid_0__Fastvid_zigzag_match__1_splitter___redArg(lean_object*, lean_object*, lean_object*);
+LEAN_EXPORT lean_object* l_Fastvid_parallelRiceLanes;
 LEAN_EXPORT lean_object* l_Fastvid_unzigzag(lean_object*);
 LEAN_EXPORT lean_object* l_Fastvid_fixedWidthModulus(lean_object*);
 LEAN_EXPORT lean_object* l_Fastvid_ransSlot(lean_object*, lean_object*);
 static lean_object* l_Fastvid_instReprPredictionMode___closed__0;
 LEAN_EXPORT lean_object* l_Fastvid_PredictionMode_ofNat___boxed(lean_object*);
 LEAN_EXPORT lean_object* l_Fastvid_ransTableSize___boxed(lean_object*);
+LEAN_EXPORT lean_object* l_Fastvid_parallelBandRows;
 LEAN_EXPORT lean_object* l_Fastvid_riceRemainder(lean_object*, lean_object*);
 static lean_object* l_Fastvid_reprPredictionMode___closed__8____x40_Fastvid___hyg_406_;
 LEAN_EXPORT lean_object* l_Fastvid_riceQuotient___boxed(lean_object*, lean_object*);
@@ -67,10 +75,13 @@ LEAN_EXPORT lean_object* l_Fastvid_PredictionMode_noConfusion___redArg___lam__0_
 static lean_object* l_Fastvid_reprPredictionMode___closed__10____x40_Fastvid___hyg_406_;
 LEAN_EXPORT lean_object* l_Fastvid_instReprPredictionMode;
 lean_object* lean_nat_abs(lean_object*);
+LEAN_EXPORT lean_object* l_Fastvid_predictorBandRow(lean_object*);
+LEAN_EXPORT lean_object* l_Fastvid_predictorBandIndex___boxed(lean_object*);
 lean_object* lean_nat_pow(lean_object*, lean_object*);
 LEAN_EXPORT lean_object* l_Fastvid_sampleMax(lean_object*);
 uint8_t lean_nat_dec_eq(lean_object*, lean_object*);
 LEAN_EXPORT lean_object* l_Fastvid_unzigzag___boxed(lean_object*);
+LEAN_EXPORT lean_object* l_Fastvid_predictorBandRow___boxed(lean_object*);
 lean_object* lean_nat_mod(lean_object*, lean_object*);
 LEAN_EXPORT lean_object* l_Fastvid_PredictionMode_noConfusion(lean_object*, uint8_t, uint8_t, lean_object*);
 static lean_object* l_Fastvid_reprPredictionMode___closed__5____x40_Fastvid___hyg_406_;
@@ -84,6 +95,7 @@ lean_object* lean_nat_mul(lean_object*, lean_object*);
 lean_object* lean_int_neg_succ_of_nat(lean_object*);
 static lean_object* l_Fastvid_reprPredictionMode___closed__11____x40_Fastvid___hyg_406_;
 static lean_object* l_Fastvid_zigzag___closed__0;
+static lean_object* l_Fastvid_maximumParallelBlockBodyBytes___closed__1;
 LEAN_EXPORT lean_object* l___private_Fastvid_0__Fastvid_zigzag_match__1_splitter(lean_object*, lean_object*, lean_object*, lean_object*);
 LEAN_EXPORT lean_object* l_Fastvid_ransStateIndex___boxed(lean_object*, lean_object*);
 LEAN_EXPORT uint8_t l_Fastvid_PredictionMode_ofNat(lean_object*);
@@ -93,14 +105,16 @@ LEAN_EXPORT lean_object* l_Fastvid_zigzag(lean_object*);
 lean_object* lean_nat_add(lean_object*, lean_object*);
 LEAN_EXPORT lean_object* l_Fastvid_clampSample___boxed(lean_object*, lean_object*);
 LEAN_EXPORT lean_object* l_Fastvid_PredictionMode_noConfusion___redArg(uint8_t, uint8_t);
+LEAN_EXPORT lean_object* l_Fastvid_maximumParallelBlockBodyBytes;
 static lean_object* l_Fastvid_reprPredictionMode___closed__7____x40_Fastvid___hyg_406_;
 LEAN_EXPORT lean_object* l_Fastvid_PredictionMode_toCtorIdx___boxed(lean_object*);
 LEAN_EXPORT lean_object* l_Fastvid_temporalResidual(lean_object*, lean_object*);
 LEAN_EXPORT lean_object* l_Fastvid_ransDecodeState___boxed(lean_object*, lean_object*, lean_object*, lean_object*);
+static lean_object* l_Fastvid_maximumParallelBlockBodyBytes___closed__2;
 static lean_object* _init_l_Fastvid_zigzag___closed__0() {
 _start:
 {
-lean_object* x_1; lean_object* x_2; 
+lean_object* x_1; lean_object* x_2;
 x_1 = lean_unsigned_to_nat(0u);
 x_2 = lean_nat_to_int(x_1);
 return x_2;
@@ -109,12 +123,12 @@ return x_2;
 LEAN_EXPORT lean_object* l_Fastvid_zigzag(lean_object* x_1) {
 _start:
 {
-lean_object* x_2; uint8_t x_3; 
+lean_object* x_2; uint8_t x_3;
 x_2 = l_Fastvid_zigzag___closed__0;
 x_3 = lean_int_dec_lt(x_1, x_2);
 if (x_3 == 0)
 {
-lean_object* x_4; lean_object* x_5; lean_object* x_6; 
+lean_object* x_4; lean_object* x_5; lean_object* x_6;
 x_4 = lean_nat_abs(x_1);
 x_5 = lean_unsigned_to_nat(2u);
 x_6 = lean_nat_mul(x_5, x_4);
@@ -123,7 +137,7 @@ return x_6;
 }
 else
 {
-lean_object* x_7; lean_object* x_8; lean_object* x_9; lean_object* x_10; lean_object* x_11; lean_object* x_12; 
+lean_object* x_7; lean_object* x_8; lean_object* x_9; lean_object* x_10; lean_object* x_11; lean_object* x_12;
 x_7 = lean_nat_abs(x_1);
 x_8 = lean_unsigned_to_nat(1u);
 x_9 = lean_nat_sub(x_7, x_8);
@@ -140,7 +154,7 @@ return x_12;
 LEAN_EXPORT lean_object* l_Fastvid_zigzag___boxed(lean_object* x_1) {
 _start:
 {
-lean_object* x_2; 
+lean_object* x_2;
 x_2 = l_Fastvid_zigzag(x_1);
 lean_dec(x_1);
 return x_2;
@@ -149,7 +163,7 @@ return x_2;
 LEAN_EXPORT lean_object* l_Fastvid_unzigzag(lean_object* x_1) {
 _start:
 {
-lean_object* x_2; lean_object* x_3; lean_object* x_4; uint8_t x_5; 
+lean_object* x_2; lean_object* x_3; lean_object* x_4; uint8_t x_5;
 x_2 = lean_unsigned_to_nat(2u);
 x_3 = lean_nat_mod(x_1, x_2);
 x_4 = lean_unsigned_to_nat(0u);
@@ -157,7 +171,7 @@ x_5 = lean_nat_dec_eq(x_3, x_4);
 lean_dec(x_3);
 if (x_5 == 0)
 {
-lean_object* x_6; lean_object* x_7; lean_object* x_8; 
+lean_object* x_6; lean_object* x_7; lean_object* x_8;
 x_6 = lean_unsigned_to_nat(1u);
 x_7 = lean_nat_shiftr(x_1, x_6);
 x_8 = lean_int_neg_succ_of_nat(x_7);
@@ -165,7 +179,7 @@ return x_8;
 }
 else
 {
-lean_object* x_9; lean_object* x_10; lean_object* x_11; 
+lean_object* x_9; lean_object* x_10; lean_object* x_11;
 x_9 = lean_unsigned_to_nat(1u);
 x_10 = lean_nat_shiftr(x_1, x_9);
 x_11 = lean_nat_to_int(x_10);
@@ -176,7 +190,7 @@ return x_11;
 LEAN_EXPORT lean_object* l_Fastvid_unzigzag___boxed(lean_object* x_1) {
 _start:
 {
-lean_object* x_2; 
+lean_object* x_2;
 x_2 = l_Fastvid_unzigzag(x_1);
 lean_dec(x_1);
 return x_2;
@@ -185,7 +199,7 @@ return x_2;
 static lean_object* _init_l___private_Fastvid_0__Fastvid_zigzag_match__1_splitter___redArg___closed__0() {
 _start:
 {
-lean_object* x_1; lean_object* x_2; 
+lean_object* x_1; lean_object* x_2;
 x_1 = lean_unsigned_to_nat(0u);
 x_2 = lean_nat_to_int(x_1);
 return x_2;
@@ -194,12 +208,12 @@ return x_2;
 LEAN_EXPORT lean_object* l___private_Fastvid_0__Fastvid_zigzag_match__1_splitter___redArg(lean_object* x_1, lean_object* x_2, lean_object* x_3) {
 _start:
 {
-lean_object* x_4; uint8_t x_5; 
+lean_object* x_4; uint8_t x_5;
 x_4 = l___private_Fastvid_0__Fastvid_zigzag_match__1_splitter___redArg___closed__0;
 x_5 = lean_int_dec_lt(x_1, x_4);
 if (x_5 == 0)
 {
-lean_object* x_6; lean_object* x_7; 
+lean_object* x_6; lean_object* x_7;
 lean_dec(x_3);
 x_6 = lean_nat_abs(x_1);
 x_7 = lean_apply_1(x_2, x_6);
@@ -207,7 +221,7 @@ return x_7;
 }
 else
 {
-lean_object* x_8; lean_object* x_9; lean_object* x_10; lean_object* x_11; 
+lean_object* x_8; lean_object* x_9; lean_object* x_10; lean_object* x_11;
 lean_dec(x_2);
 x_8 = lean_nat_abs(x_1);
 x_9 = lean_unsigned_to_nat(1u);
@@ -221,7 +235,7 @@ return x_11;
 LEAN_EXPORT lean_object* l___private_Fastvid_0__Fastvid_zigzag_match__1_splitter(lean_object* x_1, lean_object* x_2, lean_object* x_3, lean_object* x_4) {
 _start:
 {
-lean_object* x_5; 
+lean_object* x_5;
 x_5 = l___private_Fastvid_0__Fastvid_zigzag_match__1_splitter___redArg(x_2, x_3, x_4);
 return x_5;
 }
@@ -229,7 +243,7 @@ return x_5;
 LEAN_EXPORT lean_object* l___private_Fastvid_0__Fastvid_zigzag_match__1_splitter___redArg___boxed(lean_object* x_1, lean_object* x_2, lean_object* x_3) {
 _start:
 {
-lean_object* x_4; 
+lean_object* x_4;
 x_4 = l___private_Fastvid_0__Fastvid_zigzag_match__1_splitter___redArg(x_1, x_2, x_3);
 lean_dec(x_1);
 return x_4;
@@ -238,7 +252,7 @@ return x_4;
 LEAN_EXPORT lean_object* l___private_Fastvid_0__Fastvid_zigzag_match__1_splitter___boxed(lean_object* x_1, lean_object* x_2, lean_object* x_3, lean_object* x_4) {
 _start:
 {
-lean_object* x_5; 
+lean_object* x_5;
 x_5 = l___private_Fastvid_0__Fastvid_zigzag_match__1_splitter(x_1, x_2, x_3, x_4);
 lean_dec(x_2);
 return x_5;
@@ -247,7 +261,7 @@ return x_5;
 LEAN_EXPORT lean_object* l_Fastvid_riceDivisor(lean_object* x_1) {
 _start:
 {
-lean_object* x_2; lean_object* x_3; 
+lean_object* x_2; lean_object* x_3;
 x_2 = lean_unsigned_to_nat(2u);
 x_3 = lean_nat_pow(x_2, x_1);
 return x_3;
@@ -256,7 +270,7 @@ return x_3;
 LEAN_EXPORT lean_object* l_Fastvid_riceDivisor___boxed(lean_object* x_1) {
 _start:
 {
-lean_object* x_2; 
+lean_object* x_2;
 x_2 = l_Fastvid_riceDivisor(x_1);
 lean_dec(x_1);
 return x_2;
@@ -265,7 +279,7 @@ return x_2;
 LEAN_EXPORT lean_object* l_Fastvid_riceQuotient(lean_object* x_1, lean_object* x_2) {
 _start:
 {
-lean_object* x_3; lean_object* x_4; 
+lean_object* x_3; lean_object* x_4;
 x_3 = l_Fastvid_riceDivisor(x_2);
 x_4 = lean_nat_div(x_1, x_3);
 lean_dec(x_3);
@@ -275,7 +289,7 @@ return x_4;
 LEAN_EXPORT lean_object* l_Fastvid_riceQuotient___boxed(lean_object* x_1, lean_object* x_2) {
 _start:
 {
-lean_object* x_3; 
+lean_object* x_3;
 x_3 = l_Fastvid_riceQuotient(x_1, x_2);
 lean_dec(x_2);
 lean_dec(x_1);
@@ -285,7 +299,7 @@ return x_3;
 LEAN_EXPORT lean_object* l_Fastvid_riceRemainder(lean_object* x_1, lean_object* x_2) {
 _start:
 {
-lean_object* x_3; lean_object* x_4; 
+lean_object* x_3; lean_object* x_4;
 x_3 = l_Fastvid_riceDivisor(x_2);
 x_4 = lean_nat_mod(x_1, x_3);
 lean_dec(x_3);
@@ -295,7 +309,7 @@ return x_4;
 LEAN_EXPORT lean_object* l_Fastvid_riceRemainder___boxed(lean_object* x_1, lean_object* x_2) {
 _start:
 {
-lean_object* x_3; 
+lean_object* x_3;
 x_3 = l_Fastvid_riceRemainder(x_1, x_2);
 lean_dec(x_2);
 lean_dec(x_1);
@@ -305,7 +319,7 @@ return x_3;
 LEAN_EXPORT lean_object* l_Fastvid_fixedWidthModulus(lean_object* x_1) {
 _start:
 {
-lean_object* x_2; lean_object* x_3; 
+lean_object* x_2; lean_object* x_3;
 x_2 = lean_unsigned_to_nat(2u);
 x_3 = lean_nat_pow(x_2, x_1);
 return x_3;
@@ -314,7 +328,7 @@ return x_3;
 LEAN_EXPORT lean_object* l_Fastvid_fixedWidthModulus___boxed(lean_object* x_1) {
 _start:
 {
-lean_object* x_2; 
+lean_object* x_2;
 x_2 = l_Fastvid_fixedWidthModulus(x_1);
 lean_dec(x_1);
 return x_2;
@@ -323,7 +337,7 @@ return x_2;
 LEAN_EXPORT lean_object* l_Fastvid_temporalResidual(lean_object* x_1, lean_object* x_2) {
 _start:
 {
-lean_object* x_3; 
+lean_object* x_3;
 x_3 = lean_int_sub(x_1, x_2);
 return x_3;
 }
@@ -331,7 +345,7 @@ return x_3;
 LEAN_EXPORT lean_object* l_Fastvid_temporalResidual___boxed(lean_object* x_1, lean_object* x_2) {
 _start:
 {
-lean_object* x_3; 
+lean_object* x_3;
 x_3 = l_Fastvid_temporalResidual(x_1, x_2);
 lean_dec(x_2);
 lean_dec(x_1);
@@ -341,7 +355,7 @@ return x_3;
 LEAN_EXPORT lean_object* l_Fastvid_sampleMax(lean_object* x_1) {
 _start:
 {
-lean_object* x_2; lean_object* x_3; lean_object* x_4; lean_object* x_5; 
+lean_object* x_2; lean_object* x_3; lean_object* x_4; lean_object* x_5;
 x_2 = lean_unsigned_to_nat(2u);
 x_3 = lean_nat_pow(x_2, x_1);
 x_4 = lean_unsigned_to_nat(1u);
@@ -353,7 +367,7 @@ return x_5;
 LEAN_EXPORT lean_object* l_Fastvid_sampleMax___boxed(lean_object* x_1) {
 _start:
 {
-lean_object* x_2; 
+lean_object* x_2;
 x_2 = l_Fastvid_sampleMax(x_1);
 lean_dec(x_1);
 return x_2;
@@ -362,7 +376,7 @@ return x_2;
 LEAN_EXPORT lean_object* l_Fastvid_quantStep(lean_object* x_1, lean_object* x_2) {
 _start:
 {
-lean_object* x_3; lean_object* x_4; lean_object* x_5; lean_object* x_6; lean_object* x_7; lean_object* x_8; lean_object* x_9; lean_object* x_10; lean_object* x_11; lean_object* x_12; lean_object* x_13; 
+lean_object* x_3; lean_object* x_4; lean_object* x_5; lean_object* x_6; lean_object* x_7; lean_object* x_8; lean_object* x_9; lean_object* x_10; lean_object* x_11; lean_object* x_12; lean_object* x_13;
 x_3 = lean_unsigned_to_nat(1u);
 x_4 = lean_unsigned_to_nat(100u);
 x_5 = lean_nat_sub(x_4, x_1);
@@ -385,7 +399,7 @@ return x_13;
 LEAN_EXPORT lean_object* l_Fastvid_quantStep___boxed(lean_object* x_1, lean_object* x_2) {
 _start:
 {
-lean_object* x_3; 
+lean_object* x_3;
 x_3 = l_Fastvid_quantStep(x_1, x_2);
 lean_dec(x_2);
 lean_dec(x_1);
@@ -398,31 +412,31 @@ _start:
 switch (x_1) {
 case 0:
 {
-lean_object* x_2; 
+lean_object* x_2;
 x_2 = lean_unsigned_to_nat(0u);
 return x_2;
 }
 case 1:
 {
-lean_object* x_3; 
+lean_object* x_3;
 x_3 = lean_unsigned_to_nat(1u);
 return x_3;
 }
 case 2:
 {
-lean_object* x_4; 
+lean_object* x_4;
 x_4 = lean_unsigned_to_nat(2u);
 return x_4;
 }
 case 3:
 {
-lean_object* x_5; 
+lean_object* x_5;
 x_5 = lean_unsigned_to_nat(3u);
 return x_5;
 }
-default: 
+default:
 {
-lean_object* x_6; 
+lean_object* x_6;
 x_6 = lean_unsigned_to_nat(4u);
 return x_6;
 }
@@ -432,7 +446,7 @@ return x_6;
 LEAN_EXPORT lean_object* l_Fastvid_PredictionMode_toCtorIdx___boxed(lean_object* x_1) {
 _start:
 {
-uint8_t x_2; lean_object* x_3; 
+uint8_t x_2; lean_object* x_3;
 x_2 = lean_unbox(x_1);
 lean_dec(x_1);
 x_3 = l_Fastvid_PredictionMode_toCtorIdx(x_2);
@@ -449,7 +463,7 @@ return x_1;
 LEAN_EXPORT lean_object* l_Fastvid_PredictionMode_noConfusion___redArg(uint8_t x_1, uint8_t x_2) {
 _start:
 {
-lean_object* x_3; 
+lean_object* x_3;
 x_3 = lean_alloc_closure((void*)(l_Fastvid_PredictionMode_noConfusion___redArg___lam__0___boxed), 1, 0);
 return x_3;
 }
@@ -457,7 +471,7 @@ return x_3;
 LEAN_EXPORT lean_object* l_Fastvid_PredictionMode_noConfusion(lean_object* x_1, uint8_t x_2, uint8_t x_3, lean_object* x_4) {
 _start:
 {
-lean_object* x_5; 
+lean_object* x_5;
 x_5 = l_Fastvid_PredictionMode_noConfusion___redArg(x_2, x_3);
 return x_5;
 }
@@ -465,7 +479,7 @@ return x_5;
 LEAN_EXPORT lean_object* l_Fastvid_PredictionMode_noConfusion___redArg___lam__0___boxed(lean_object* x_1) {
 _start:
 {
-lean_object* x_2; 
+lean_object* x_2;
 x_2 = l_Fastvid_PredictionMode_noConfusion___redArg___lam__0(x_1);
 lean_dec(x_1);
 return x_2;
@@ -474,7 +488,7 @@ return x_2;
 LEAN_EXPORT lean_object* l_Fastvid_PredictionMode_noConfusion___redArg___boxed(lean_object* x_1, lean_object* x_2) {
 _start:
 {
-uint8_t x_3; uint8_t x_4; lean_object* x_5; 
+uint8_t x_3; uint8_t x_4; lean_object* x_5;
 x_3 = lean_unbox(x_1);
 lean_dec(x_1);
 x_4 = lean_unbox(x_2);
@@ -486,7 +500,7 @@ return x_5;
 LEAN_EXPORT lean_object* l_Fastvid_PredictionMode_noConfusion___boxed(lean_object* x_1, lean_object* x_2, lean_object* x_3, lean_object* x_4) {
 _start:
 {
-uint8_t x_5; uint8_t x_6; lean_object* x_7; 
+uint8_t x_5; uint8_t x_6; lean_object* x_7;
 x_5 = lean_unbox(x_2);
 lean_dec(x_2);
 x_6 = lean_unbox(x_3);
@@ -498,24 +512,24 @@ return x_7;
 LEAN_EXPORT uint8_t l_Fastvid_PredictionMode_ofNat(lean_object* x_1) {
 _start:
 {
-lean_object* x_2; uint8_t x_3; 
+lean_object* x_2; uint8_t x_3;
 x_2 = lean_unsigned_to_nat(2u);
 x_3 = lean_nat_dec_le(x_2, x_1);
 if (x_3 == 0)
 {
-lean_object* x_4; uint8_t x_5; 
+lean_object* x_4; uint8_t x_5;
 x_4 = lean_unsigned_to_nat(0u);
 x_5 = lean_nat_dec_eq(x_1, x_4);
 if (x_5 == 0)
 {
-lean_object* x_6; uint8_t x_7; 
+lean_object* x_6; uint8_t x_7;
 x_6 = lean_box(1);
 x_7 = lean_unbox(x_6);
 return x_7;
 }
 else
 {
-lean_object* x_8; uint8_t x_9; 
+lean_object* x_8; uint8_t x_9;
 x_8 = lean_box(0);
 x_9 = lean_unbox(x_8);
 return x_9;
@@ -523,30 +537,30 @@ return x_9;
 }
 else
 {
-lean_object* x_10; uint8_t x_11; 
+lean_object* x_10; uint8_t x_11;
 x_10 = lean_unsigned_to_nat(3u);
 x_11 = lean_nat_dec_le(x_10, x_1);
 if (x_11 == 0)
 {
-lean_object* x_12; uint8_t x_13; 
+lean_object* x_12; uint8_t x_13;
 x_12 = lean_box(2);
 x_13 = lean_unbox(x_12);
 return x_13;
 }
 else
 {
-uint8_t x_14; 
+uint8_t x_14;
 x_14 = lean_nat_dec_eq(x_1, x_10);
 if (x_14 == 0)
 {
-lean_object* x_15; uint8_t x_16; 
+lean_object* x_15; uint8_t x_16;
 x_15 = lean_box(4);
 x_16 = lean_unbox(x_15);
 return x_16;
 }
 else
 {
-lean_object* x_17; uint8_t x_18; 
+lean_object* x_17; uint8_t x_18;
 x_17 = lean_box(3);
 x_18 = lean_unbox(x_17);
 return x_18;
@@ -558,7 +572,7 @@ return x_18;
 LEAN_EXPORT lean_object* l_Fastvid_PredictionMode_ofNat___boxed(lean_object* x_1) {
 _start:
 {
-uint8_t x_2; lean_object* x_3; 
+uint8_t x_2; lean_object* x_3;
 x_2 = l_Fastvid_PredictionMode_ofNat(x_1);
 lean_dec(x_1);
 x_3 = lean_box(x_2);
@@ -568,7 +582,7 @@ return x_3;
 LEAN_EXPORT uint8_t l_Fastvid_instDecidableEqPredictionMode(uint8_t x_1, uint8_t x_2) {
 _start:
 {
-lean_object* x_3; lean_object* x_4; uint8_t x_5; 
+lean_object* x_3; lean_object* x_4; uint8_t x_5;
 x_3 = l_Fastvid_PredictionMode_toCtorIdx(x_1);
 x_4 = l_Fastvid_PredictionMode_toCtorIdx(x_2);
 x_5 = lean_nat_dec_eq(x_3, x_4);
@@ -580,7 +594,7 @@ return x_5;
 LEAN_EXPORT lean_object* l_Fastvid_instDecidableEqPredictionMode___boxed(lean_object* x_1, lean_object* x_2) {
 _start:
 {
-uint8_t x_3; uint8_t x_4; uint8_t x_5; lean_object* x_6; 
+uint8_t x_3; uint8_t x_4; uint8_t x_5; lean_object* x_6;
 x_3 = lean_unbox(x_1);
 lean_dec(x_1);
 x_4 = lean_unbox(x_2);
@@ -593,7 +607,7 @@ return x_6;
 static lean_object* _init_l_Fastvid_reprPredictionMode___closed__0____x40_Fastvid___hyg_406_() {
 _start:
 {
-lean_object* x_1; 
+lean_object* x_1;
 x_1 = lean_mk_string_unchecked("Fastvid.PredictionMode.paeth", 28, 28);
 return x_1;
 }
@@ -601,7 +615,7 @@ return x_1;
 static lean_object* _init_l_Fastvid_reprPredictionMode___closed__1____x40_Fastvid___hyg_406_() {
 _start:
 {
-lean_object* x_1; lean_object* x_2; 
+lean_object* x_1; lean_object* x_2;
 x_1 = l_Fastvid_reprPredictionMode___closed__0____x40_Fastvid___hyg_406_;
 x_2 = lean_alloc_ctor(3, 1, 0);
 lean_ctor_set(x_2, 0, x_1);
@@ -611,7 +625,7 @@ return x_2;
 static lean_object* _init_l_Fastvid_reprPredictionMode___closed__2____x40_Fastvid___hyg_406_() {
 _start:
 {
-lean_object* x_1; 
+lean_object* x_1;
 x_1 = lean_mk_string_unchecked("Fastvid.PredictionMode.temporal", 31, 31);
 return x_1;
 }
@@ -619,7 +633,7 @@ return x_1;
 static lean_object* _init_l_Fastvid_reprPredictionMode___closed__3____x40_Fastvid___hyg_406_() {
 _start:
 {
-lean_object* x_1; lean_object* x_2; 
+lean_object* x_1; lean_object* x_2;
 x_1 = l_Fastvid_reprPredictionMode___closed__2____x40_Fastvid___hyg_406_;
 x_2 = lean_alloc_ctor(3, 1, 0);
 lean_ctor_set(x_2, 0, x_1);
@@ -629,7 +643,7 @@ return x_2;
 static lean_object* _init_l_Fastvid_reprPredictionMode___closed__4____x40_Fastvid___hyg_406_() {
 _start:
 {
-lean_object* x_1; 
+lean_object* x_1;
 x_1 = lean_mk_string_unchecked("Fastvid.PredictionMode.average", 30, 30);
 return x_1;
 }
@@ -637,7 +651,7 @@ return x_1;
 static lean_object* _init_l_Fastvid_reprPredictionMode___closed__5____x40_Fastvid___hyg_406_() {
 _start:
 {
-lean_object* x_1; lean_object* x_2; 
+lean_object* x_1; lean_object* x_2;
 x_1 = l_Fastvid_reprPredictionMode___closed__4____x40_Fastvid___hyg_406_;
 x_2 = lean_alloc_ctor(3, 1, 0);
 lean_ctor_set(x_2, 0, x_1);
@@ -647,7 +661,7 @@ return x_2;
 static lean_object* _init_l_Fastvid_reprPredictionMode___closed__6____x40_Fastvid___hyg_406_() {
 _start:
 {
-lean_object* x_1; 
+lean_object* x_1;
 x_1 = lean_mk_string_unchecked("Fastvid.PredictionMode.clampGradient", 36, 36);
 return x_1;
 }
@@ -655,7 +669,7 @@ return x_1;
 static lean_object* _init_l_Fastvid_reprPredictionMode___closed__7____x40_Fastvid___hyg_406_() {
 _start:
 {
-lean_object* x_1; lean_object* x_2; 
+lean_object* x_1; lean_object* x_2;
 x_1 = l_Fastvid_reprPredictionMode___closed__6____x40_Fastvid___hyg_406_;
 x_2 = lean_alloc_ctor(3, 1, 0);
 lean_ctor_set(x_2, 0, x_1);
@@ -665,7 +679,7 @@ return x_2;
 static lean_object* _init_l_Fastvid_reprPredictionMode___closed__8____x40_Fastvid___hyg_406_() {
 _start:
 {
-lean_object* x_1; 
+lean_object* x_1;
 x_1 = lean_mk_string_unchecked("Fastvid.PredictionMode.halfGradient", 35, 35);
 return x_1;
 }
@@ -673,7 +687,7 @@ return x_1;
 static lean_object* _init_l_Fastvid_reprPredictionMode___closed__9____x40_Fastvid___hyg_406_() {
 _start:
 {
-lean_object* x_1; lean_object* x_2; 
+lean_object* x_1; lean_object* x_2;
 x_1 = l_Fastvid_reprPredictionMode___closed__8____x40_Fastvid___hyg_406_;
 x_2 = lean_alloc_ctor(3, 1, 0);
 lean_ctor_set(x_2, 0, x_1);
@@ -683,7 +697,7 @@ return x_2;
 static lean_object* _init_l_Fastvid_reprPredictionMode___closed__10____x40_Fastvid___hyg_406_() {
 _start:
 {
-lean_object* x_1; lean_object* x_2; 
+lean_object* x_1; lean_object* x_2;
 x_1 = lean_unsigned_to_nat(2u);
 x_2 = lean_nat_to_int(x_1);
 return x_2;
@@ -692,7 +706,7 @@ return x_2;
 static lean_object* _init_l_Fastvid_reprPredictionMode___closed__11____x40_Fastvid___hyg_406_() {
 _start:
 {
-lean_object* x_1; lean_object* x_2; 
+lean_object* x_1; lean_object* x_2;
 x_1 = lean_unsigned_to_nat(1u);
 x_2 = lean_nat_to_int(x_1);
 return x_2;
@@ -701,23 +715,23 @@ return x_2;
 LEAN_EXPORT lean_object* l_Fastvid_reprPredictionMode____x40_Fastvid___hyg_406_(uint8_t x_1, lean_object* x_2) {
 _start:
 {
-lean_object* x_3; lean_object* x_11; lean_object* x_19; lean_object* x_27; lean_object* x_35; 
+lean_object* x_3; lean_object* x_11; lean_object* x_19; lean_object* x_27; lean_object* x_35;
 switch (x_1) {
 case 0:
 {
-lean_object* x_43; uint8_t x_44; 
+lean_object* x_43; uint8_t x_44;
 x_43 = lean_unsigned_to_nat(1024u);
 x_44 = lean_nat_dec_le(x_43, x_2);
 if (x_44 == 0)
 {
-lean_object* x_45; 
+lean_object* x_45;
 x_45 = l_Fastvid_reprPredictionMode___closed__10____x40_Fastvid___hyg_406_;
 x_3 = x_45;
 goto block_10;
 }
 else
 {
-lean_object* x_46; 
+lean_object* x_46;
 x_46 = l_Fastvid_reprPredictionMode___closed__11____x40_Fastvid___hyg_406_;
 x_3 = x_46;
 goto block_10;
@@ -725,19 +739,19 @@ goto block_10;
 }
 case 1:
 {
-lean_object* x_47; uint8_t x_48; 
+lean_object* x_47; uint8_t x_48;
 x_47 = lean_unsigned_to_nat(1024u);
 x_48 = lean_nat_dec_le(x_47, x_2);
 if (x_48 == 0)
 {
-lean_object* x_49; 
+lean_object* x_49;
 x_49 = l_Fastvid_reprPredictionMode___closed__10____x40_Fastvid___hyg_406_;
 x_11 = x_49;
 goto block_18;
 }
 else
 {
-lean_object* x_50; 
+lean_object* x_50;
 x_50 = l_Fastvid_reprPredictionMode___closed__11____x40_Fastvid___hyg_406_;
 x_11 = x_50;
 goto block_18;
@@ -745,19 +759,19 @@ goto block_18;
 }
 case 2:
 {
-lean_object* x_51; uint8_t x_52; 
+lean_object* x_51; uint8_t x_52;
 x_51 = lean_unsigned_to_nat(1024u);
 x_52 = lean_nat_dec_le(x_51, x_2);
 if (x_52 == 0)
 {
-lean_object* x_53; 
+lean_object* x_53;
 x_53 = l_Fastvid_reprPredictionMode___closed__10____x40_Fastvid___hyg_406_;
 x_19 = x_53;
 goto block_26;
 }
 else
 {
-lean_object* x_54; 
+lean_object* x_54;
 x_54 = l_Fastvid_reprPredictionMode___closed__11____x40_Fastvid___hyg_406_;
 x_19 = x_54;
 goto block_26;
@@ -765,39 +779,39 @@ goto block_26;
 }
 case 3:
 {
-lean_object* x_55; uint8_t x_56; 
+lean_object* x_55; uint8_t x_56;
 x_55 = lean_unsigned_to_nat(1024u);
 x_56 = lean_nat_dec_le(x_55, x_2);
 if (x_56 == 0)
 {
-lean_object* x_57; 
+lean_object* x_57;
 x_57 = l_Fastvid_reprPredictionMode___closed__10____x40_Fastvid___hyg_406_;
 x_27 = x_57;
 goto block_34;
 }
 else
 {
-lean_object* x_58; 
+lean_object* x_58;
 x_58 = l_Fastvid_reprPredictionMode___closed__11____x40_Fastvid___hyg_406_;
 x_27 = x_58;
 goto block_34;
 }
 }
-default: 
+default:
 {
-lean_object* x_59; uint8_t x_60; 
+lean_object* x_59; uint8_t x_60;
 x_59 = lean_unsigned_to_nat(1024u);
 x_60 = lean_nat_dec_le(x_59, x_2);
 if (x_60 == 0)
 {
-lean_object* x_61; 
+lean_object* x_61;
 x_61 = l_Fastvid_reprPredictionMode___closed__10____x40_Fastvid___hyg_406_;
 x_35 = x_61;
 goto block_42;
 }
 else
 {
-lean_object* x_62; 
+lean_object* x_62;
 x_62 = l_Fastvid_reprPredictionMode___closed__11____x40_Fastvid___hyg_406_;
 x_35 = x_62;
 goto block_42;
@@ -806,7 +820,7 @@ goto block_42;
 }
 block_10:
 {
-lean_object* x_4; lean_object* x_5; lean_object* x_6; lean_object* x_7; uint8_t x_8; lean_object* x_9; 
+lean_object* x_4; lean_object* x_5; lean_object* x_6; lean_object* x_7; uint8_t x_8; lean_object* x_9;
 x_4 = l_Fastvid_reprPredictionMode___closed__1____x40_Fastvid___hyg_406_;
 x_5 = lean_alloc_ctor(4, 2, 0);
 lean_ctor_set(x_5, 0, x_3);
@@ -821,7 +835,7 @@ return x_9;
 }
 block_18:
 {
-lean_object* x_12; lean_object* x_13; lean_object* x_14; lean_object* x_15; uint8_t x_16; lean_object* x_17; 
+lean_object* x_12; lean_object* x_13; lean_object* x_14; lean_object* x_15; uint8_t x_16; lean_object* x_17;
 x_12 = l_Fastvid_reprPredictionMode___closed__3____x40_Fastvid___hyg_406_;
 x_13 = lean_alloc_ctor(4, 2, 0);
 lean_ctor_set(x_13, 0, x_11);
@@ -836,7 +850,7 @@ return x_17;
 }
 block_26:
 {
-lean_object* x_20; lean_object* x_21; lean_object* x_22; lean_object* x_23; uint8_t x_24; lean_object* x_25; 
+lean_object* x_20; lean_object* x_21; lean_object* x_22; lean_object* x_23; uint8_t x_24; lean_object* x_25;
 x_20 = l_Fastvid_reprPredictionMode___closed__5____x40_Fastvid___hyg_406_;
 x_21 = lean_alloc_ctor(4, 2, 0);
 lean_ctor_set(x_21, 0, x_19);
@@ -851,7 +865,7 @@ return x_25;
 }
 block_34:
 {
-lean_object* x_28; lean_object* x_29; lean_object* x_30; lean_object* x_31; uint8_t x_32; lean_object* x_33; 
+lean_object* x_28; lean_object* x_29; lean_object* x_30; lean_object* x_31; uint8_t x_32; lean_object* x_33;
 x_28 = l_Fastvid_reprPredictionMode___closed__7____x40_Fastvid___hyg_406_;
 x_29 = lean_alloc_ctor(4, 2, 0);
 lean_ctor_set(x_29, 0, x_27);
@@ -866,7 +880,7 @@ return x_33;
 }
 block_42:
 {
-lean_object* x_36; lean_object* x_37; lean_object* x_38; lean_object* x_39; uint8_t x_40; lean_object* x_41; 
+lean_object* x_36; lean_object* x_37; lean_object* x_38; lean_object* x_39; uint8_t x_40; lean_object* x_41;
 x_36 = l_Fastvid_reprPredictionMode___closed__9____x40_Fastvid___hyg_406_;
 x_37 = lean_alloc_ctor(4, 2, 0);
 lean_ctor_set(x_37, 0, x_35);
@@ -884,7 +898,7 @@ return x_41;
 LEAN_EXPORT lean_object* l_Fastvid_reprPredictionMode____x40_Fastvid___hyg_406____boxed(lean_object* x_1, lean_object* x_2) {
 _start:
 {
-uint8_t x_3; lean_object* x_4; 
+uint8_t x_3; lean_object* x_4;
 x_3 = lean_unbox(x_1);
 lean_dec(x_1);
 x_4 = l_Fastvid_reprPredictionMode____x40_Fastvid___hyg_406_(x_3, x_2);
@@ -895,7 +909,7 @@ return x_4;
 static lean_object* _init_l_Fastvid_instReprPredictionMode___closed__0() {
 _start:
 {
-lean_object* x_1; 
+lean_object* x_1;
 x_1 = lean_alloc_closure((void*)(l_Fastvid_reprPredictionMode____x40_Fastvid___hyg_406____boxed), 2, 0);
 return x_1;
 }
@@ -903,7 +917,7 @@ return x_1;
 static lean_object* _init_l_Fastvid_instReprPredictionMode() {
 _start:
 {
-lean_object* x_1; 
+lean_object* x_1;
 x_1 = l_Fastvid_instReprPredictionMode___closed__0;
 return x_1;
 }
@@ -914,31 +928,31 @@ _start:
 switch (x_1) {
 case 0:
 {
-lean_object* x_2; 
+lean_object* x_2;
 x_2 = lean_unsigned_to_nat(0u);
 return x_2;
 }
 case 1:
 {
-lean_object* x_3; 
+lean_object* x_3;
 x_3 = lean_unsigned_to_nat(1u);
 return x_3;
 }
 case 2:
 {
-lean_object* x_4; 
+lean_object* x_4;
 x_4 = lean_unsigned_to_nat(2u);
 return x_4;
 }
 case 3:
 {
-lean_object* x_5; 
+lean_object* x_5;
 x_5 = lean_unsigned_to_nat(3u);
 return x_5;
 }
-default: 
+default:
 {
-lean_object* x_6; 
+lean_object* x_6;
 x_6 = lean_unsigned_to_nat(4u);
 return x_6;
 }
@@ -948,7 +962,7 @@ return x_6;
 LEAN_EXPORT lean_object* l_Fastvid_predictionModeCode___boxed(lean_object* x_1) {
 _start:
 {
-uint8_t x_2; lean_object* x_3; 
+uint8_t x_2; lean_object* x_3;
 x_2 = lean_unbox(x_1);
 lean_dec(x_1);
 x_3 = l_Fastvid_predictionModeCode(x_2);
@@ -958,7 +972,7 @@ return x_3;
 LEAN_EXPORT lean_object* l_Fastvid_average2(lean_object* x_1, lean_object* x_2) {
 _start:
 {
-lean_object* x_3; lean_object* x_4; lean_object* x_5; 
+lean_object* x_3; lean_object* x_4; lean_object* x_5;
 x_3 = lean_nat_add(x_1, x_2);
 x_4 = lean_unsigned_to_nat(1u);
 x_5 = lean_nat_shiftr(x_3, x_4);
@@ -969,7 +983,7 @@ return x_5;
 LEAN_EXPORT lean_object* l_Fastvid_average2___boxed(lean_object* x_1, lean_object* x_2) {
 _start:
 {
-lean_object* x_3; 
+lean_object* x_3;
 x_3 = l_Fastvid_average2(x_1, x_2);
 lean_dec(x_2);
 lean_dec(x_1);
@@ -979,13 +993,13 @@ return x_3;
 LEAN_EXPORT lean_object* l_Fastvid_clampSample(lean_object* x_1, lean_object* x_2) {
 _start:
 {
-lean_object* x_3; lean_object* x_4; uint8_t x_5; 
+lean_object* x_3; lean_object* x_4; uint8_t x_5;
 x_3 = lean_unsigned_to_nat(0u);
 x_4 = l_Fastvid_zigzag___closed__0;
 x_5 = lean_int_dec_lt(x_1, x_4);
 if (x_5 == 0)
 {
-lean_object* x_6; uint8_t x_7; 
+lean_object* x_6; uint8_t x_7;
 x_6 = l_Int_toNat(x_1);
 x_7 = lean_nat_dec_le(x_6, x_2);
 if (x_7 == 0)
@@ -1008,7 +1022,7 @@ return x_3;
 LEAN_EXPORT lean_object* l_Fastvid_clampSample___boxed(lean_object* x_1, lean_object* x_2) {
 _start:
 {
-lean_object* x_3; 
+lean_object* x_3;
 x_3 = l_Fastvid_clampSample(x_1, x_2);
 lean_dec(x_2);
 lean_dec(x_1);
@@ -1018,7 +1032,7 @@ return x_3;
 LEAN_EXPORT lean_object* l_Fastvid_ransTableSize(lean_object* x_1) {
 _start:
 {
-lean_object* x_2; lean_object* x_3; 
+lean_object* x_2; lean_object* x_3;
 x_2 = lean_unsigned_to_nat(2u);
 x_3 = lean_nat_pow(x_2, x_1);
 return x_3;
@@ -1027,7 +1041,7 @@ return x_3;
 LEAN_EXPORT lean_object* l_Fastvid_ransTableSize___boxed(lean_object* x_1) {
 _start:
 {
-lean_object* x_2; 
+lean_object* x_2;
 x_2 = l_Fastvid_ransTableSize(x_1);
 lean_dec(x_1);
 return x_2;
@@ -1036,7 +1050,7 @@ return x_2;
 LEAN_EXPORT lean_object* l_Fastvid_ransSlot(lean_object* x_1, lean_object* x_2) {
 _start:
 {
-lean_object* x_3; lean_object* x_4; 
+lean_object* x_3; lean_object* x_4;
 x_3 = l_Fastvid_ransTableSize(x_2);
 x_4 = lean_nat_mod(x_1, x_3);
 lean_dec(x_3);
@@ -1046,7 +1060,7 @@ return x_4;
 LEAN_EXPORT lean_object* l_Fastvid_ransSlot___boxed(lean_object* x_1, lean_object* x_2) {
 _start:
 {
-lean_object* x_3; 
+lean_object* x_3;
 x_3 = l_Fastvid_ransSlot(x_1, x_2);
 lean_dec(x_2);
 lean_dec(x_1);
@@ -1056,7 +1070,7 @@ return x_3;
 LEAN_EXPORT lean_object* l_Fastvid_ransStateIndex(lean_object* x_1, lean_object* x_2) {
 _start:
 {
-lean_object* x_3; 
+lean_object* x_3;
 x_3 = lean_nat_mod(x_1, x_2);
 return x_3;
 }
@@ -1064,7 +1078,7 @@ return x_3;
 LEAN_EXPORT lean_object* l_Fastvid_ransStateIndex___boxed(lean_object* x_1, lean_object* x_2) {
 _start:
 {
-lean_object* x_3; 
+lean_object* x_3;
 x_3 = l_Fastvid_ransStateIndex(x_1, x_2);
 lean_dec(x_2);
 lean_dec(x_1);
@@ -1074,7 +1088,7 @@ return x_3;
 LEAN_EXPORT lean_object* l_Fastvid_ransDecodeState(lean_object* x_1, lean_object* x_2, lean_object* x_3, lean_object* x_4) {
 _start:
 {
-lean_object* x_5; lean_object* x_6; lean_object* x_7; lean_object* x_8; lean_object* x_9; lean_object* x_10; 
+lean_object* x_5; lean_object* x_6; lean_object* x_7; lean_object* x_8; lean_object* x_9; lean_object* x_10;
 x_5 = l_Fastvid_ransTableSize(x_4);
 x_6 = lean_nat_div(x_1, x_5);
 lean_dec(x_5);
@@ -1092,13 +1106,137 @@ return x_10;
 LEAN_EXPORT lean_object* l_Fastvid_ransDecodeState___boxed(lean_object* x_1, lean_object* x_2, lean_object* x_3, lean_object* x_4) {
 _start:
 {
-lean_object* x_5; 
+lean_object* x_5;
 x_5 = l_Fastvid_ransDecodeState(x_1, x_2, x_3, x_4);
 lean_dec(x_4);
 lean_dec(x_3);
 lean_dec(x_2);
 lean_dec(x_1);
 return x_5;
+}
+}
+static lean_object* _init_l_Fastvid_parallelBandRows() {
+_start:
+{
+lean_object* x_1;
+x_1 = lean_unsigned_to_nat(64u);
+return x_1;
+}
+}
+static lean_object* _init_l_Fastvid_parallelShardSymbols() {
+_start:
+{
+lean_object* x_1;
+x_1 = lean_unsigned_to_nat(4096u);
+return x_1;
+}
+}
+static lean_object* _init_l_Fastvid_parallelRiceLanes() {
+_start:
+{
+lean_object* x_1;
+x_1 = lean_unsigned_to_nat(4u);
+return x_1;
+}
+}
+LEAN_EXPORT lean_object* l_Fastvid_predictorBandIndex(lean_object* x_1) {
+_start:
+{
+lean_object* x_2; lean_object* x_3;
+x_2 = lean_unsigned_to_nat(6u);
+x_3 = lean_nat_shiftr(x_1, x_2);
+return x_3;
+}
+}
+LEAN_EXPORT lean_object* l_Fastvid_predictorBandIndex___boxed(lean_object* x_1) {
+_start:
+{
+lean_object* x_2;
+x_2 = l_Fastvid_predictorBandIndex(x_1);
+lean_dec(x_1);
+return x_2;
+}
+}
+LEAN_EXPORT lean_object* l_Fastvid_predictorBandRow(lean_object* x_1) {
+_start:
+{
+lean_object* x_2; lean_object* x_3;
+x_2 = lean_unsigned_to_nat(64u);
+x_3 = lean_nat_mod(x_1, x_2);
+return x_3;
+}
+}
+LEAN_EXPORT lean_object* l_Fastvid_predictorBandRow___boxed(lean_object* x_1) {
+_start:
+{
+lean_object* x_2;
+x_2 = l_Fastvid_predictorBandRow(x_1);
+lean_dec(x_1);
+return x_2;
+}
+}
+LEAN_EXPORT lean_object* l_Fastvid_riceLaneIndex(lean_object* x_1, lean_object* x_2) {
+_start:
+{
+lean_object* x_3;
+x_3 = lean_nat_mod(x_1, x_2);
+return x_3;
+}
+}
+LEAN_EXPORT lean_object* l_Fastvid_riceLaneIndex___boxed(lean_object* x_1, lean_object* x_2) {
+_start:
+{
+lean_object* x_3;
+x_3 = l_Fastvid_riceLaneIndex(x_1, x_2);
+lean_dec(x_2);
+lean_dec(x_1);
+return x_3;
+}
+}
+static lean_object* _init_l_Fastvid_defaultTileWavefrontRounds() {
+_start:
+{
+lean_object* x_1;
+x_1 = lean_unsigned_to_nat(383u);
+return x_1;
+}
+}
+static lean_object* _init_l_Fastvid_maximumParallelBlockBodyBytes___closed__0() {
+_start:
+{
+lean_object* x_1; lean_object* x_2; lean_object* x_3;
+x_1 = lean_unsigned_to_nat(17u);
+x_2 = lean_unsigned_to_nat(4096u);
+x_3 = lean_nat_mul(x_2, x_1);
+return x_3;
+}
+}
+static lean_object* _init_l_Fastvid_maximumParallelBlockBodyBytes___closed__1() {
+_start:
+{
+lean_object* x_1; lean_object* x_2; lean_object* x_3;
+x_1 = lean_unsigned_to_nat(3u);
+x_2 = l_Fastvid_maximumParallelBlockBodyBytes___closed__0;
+x_3 = lean_nat_shiftr(x_2, x_1);
+return x_3;
+}
+}
+static lean_object* _init_l_Fastvid_maximumParallelBlockBodyBytes___closed__2() {
+_start:
+{
+lean_object* x_1; lean_object* x_2; lean_object* x_3;
+x_1 = l_Fastvid_maximumParallelBlockBodyBytes___closed__1;
+x_2 = lean_unsigned_to_nat(32u);
+x_3 = lean_nat_add(x_2, x_1);
+return x_3;
+}
+}
+static lean_object* _init_l_Fastvid_maximumParallelBlockBodyBytes() {
+_start:
+{
+lean_object* x_1;
+x_1 = l_Fastvid_maximumParallelBlockBodyBytes___closed__2;
+return x_1;
 }
 }
 lean_object* initialize_Init(uint8_t builtin, lean_object*);
@@ -1142,6 +1280,22 @@ l_Fastvid_instReprPredictionMode___closed__0 = _init_l_Fastvid_instReprPredictio
 lean_mark_persistent(l_Fastvid_instReprPredictionMode___closed__0);
 l_Fastvid_instReprPredictionMode = _init_l_Fastvid_instReprPredictionMode();
 lean_mark_persistent(l_Fastvid_instReprPredictionMode);
+l_Fastvid_parallelBandRows = _init_l_Fastvid_parallelBandRows();
+lean_mark_persistent(l_Fastvid_parallelBandRows);
+l_Fastvid_parallelShardSymbols = _init_l_Fastvid_parallelShardSymbols();
+lean_mark_persistent(l_Fastvid_parallelShardSymbols);
+l_Fastvid_parallelRiceLanes = _init_l_Fastvid_parallelRiceLanes();
+lean_mark_persistent(l_Fastvid_parallelRiceLanes);
+l_Fastvid_defaultTileWavefrontRounds = _init_l_Fastvid_defaultTileWavefrontRounds();
+lean_mark_persistent(l_Fastvid_defaultTileWavefrontRounds);
+l_Fastvid_maximumParallelBlockBodyBytes___closed__0 = _init_l_Fastvid_maximumParallelBlockBodyBytes___closed__0();
+lean_mark_persistent(l_Fastvid_maximumParallelBlockBodyBytes___closed__0);
+l_Fastvid_maximumParallelBlockBodyBytes___closed__1 = _init_l_Fastvid_maximumParallelBlockBodyBytes___closed__1();
+lean_mark_persistent(l_Fastvid_maximumParallelBlockBodyBytes___closed__1);
+l_Fastvid_maximumParallelBlockBodyBytes___closed__2 = _init_l_Fastvid_maximumParallelBlockBodyBytes___closed__2();
+lean_mark_persistent(l_Fastvid_maximumParallelBlockBodyBytes___closed__2);
+l_Fastvid_maximumParallelBlockBodyBytes = _init_l_Fastvid_maximumParallelBlockBodyBytes();
+lean_mark_persistent(l_Fastvid_maximumParallelBlockBodyBytes);
 return lean_io_result_mk_ok(lean_box(0));
 }
 #ifdef __cplusplus
